working on termination for first translation

examples/logic/ltl/concrltl2waaScript.sml
@@ -1,4 +1,4 @@
-open HolKernel Parse bossLib boolLib gfgTheory listTheory optionTheory relationTheory
+open HolKernel Parse bossLib boolLib gfgTheory listTheory optionTheory relationTheory pred_setTheory prim_recTheory pairTheory
 
 open alterATheory sptreeTheory ltlTheory generalHelpersTheory concrRepTheory
 
@@ -15,6 +15,15 @@ val tempDNF_concr_def = Define`
   ∧ (tempDNF_concr (X f)= [[X f]])
   ∧ (tempDNF_concr (U f1 f2) = [[U f1 f2]])
   ∧ (tempDNF_concr (R f1 f2) = [[R f1 f2]])`;
+
+val props_concr_def = Define`
+    (props_concr (VAR a) = [a])
+  ∧ (props_concr (N_VAR a) = [a])
+  ∧ (props_concr (DISJ f1 f2) = props_concr f1 ++ props_concr f2)
+  ∧ (props_concr (CONJ f1 f2) = props_concr f1 ++ props_concr f2)
+  ∧ (props_concr (X f) = props_concr f)
+  ∧ (props_concr (U f1 f2) = props_concr f1 ++ props_concr f2)
+  ∧ (props_concr (R f1 f2) = props_concr f1 ++ props_concr f2)`;
 
 (* val subListsOf_def = Define` *)
 (*     (subListsOf [] = [[]]) *)
@@ -58,30 +67,99 @@ val trans_concr_def = Define`
                                            (trans_concr aP f1)))`;
 
 val expandAuto_def = Define`
-   (expandAuto [] aut = aut)
- ∧ (expandAuto (f::fs) (concrAA g init aP) =
+   (* (expandAuto φ = *)
+   (*    let initForms = tempDNF_concr φ *)
+   (*    in let a0 = concrAA empty [] (props_concr φ) *)
+   (*    in let a1 = FOLDL (\a s. addFrmlToAut a s) a0 (FLAT initForms) *)
+   (*    in let init_concr = *)
+   (*             MAP *)
+   (*                 (λ l. *)
+   (*                    MAP (\s. THE (findNode (λ(_,l). l.frml = s) a1.graph)) l) *)
+   (*                 initForms *)
+   (*    in let a_init = a1 with <| init := init_concr |> *)
+   (*    in expandAuto_step (FLAT initForms) a_init) *)
+ (expandAuto_step [] aut = aut)
+ ∧ (expandAuto_step (f::fs) (concrAA g init aP) =
      let a1 = addFrmlToAut (concrAA g init aP) f
      in let trans = trans_concr aP f
      in let allSucs = FOLDL (\pr e. e.sucs ++ pr) [] trans
      in let a2 = FOLDL (\g p. addFrmlToAut g p) a1 allSucs
      in let a3 = FOLDL (\a e. addEdgeToAut f e a) a2 trans
      in let restNodes = FILTER (\s. ~ (inAuto (concrAA g init aP) s)) allSucs
-     in expandAuto (restNodes++fs) a3)`;
+     in expandAuto_step (restNodes++fs) a3)`;
+  (qexists_tac `λ(ls,a) (ls2,a2).
+          NoNodeProcessedTwice (HD ls) (a,ls) (a2,ls2)`
+   >> rpt strip_tac
+    >- (`!g. WF (NoNodeProcessedTwice g)` suffices_by (
+           qabbrev_tac `f = 
+)
+
+[NNPT_WF])
+ )
+
+;
 
 val NoNodeProcessedTwice_def = Define`
-  NoNodeProcessedTwice g (ns,a) (ns2,a2) =
-    (({x | inAuto a2 x } ⊂ {x | inAuto a x })
-        ∧ ({x | inAuto a x } ⊆ tempSubForms g))`;
+  NoNodeProcessedTwice g (a,ns) (a2,ns2) =
+    ((tempSubForms g DIFF {x | inAuto a x }
+                  ⊂ tempSubForms g DIFF {x | inAuto a2 x })
+         \/ ((tempSubForms g DIFF {x | inAuto a x }
+              = tempSubForms g DIFF {x | inAuto a2 x })
+              ∧ ((list_size (\x. 1) ns)
+                  < (list_size (\x. 1) ns2))))`;
 
 val NNPT_WF = store_thm
  ("NNPT_WF",
   ``!g. WF (NoNodeProcessedTwice g)``,
-  fs[WF_DEF] >> rpt strip_tac
-  >> CCONTR_TAC >> fs[NoNodeProcessedTwice_def]
-
-
-)
-
+   rpt strip_tac
+   >> `WF (λ(s:α ltl_frml -> bool) t. s ⊂ t
+         ∧ s ⊆ tempSubForms g
+         ∧ t ⊆ tempSubForms g)` by (
+       `FINITE (tempSubForms g)` by metis_tac[TSF_FINITE]
+       >> metis_tac[PSUBSET_WF]
+   )
+   >> `WF ($<)` by metis_tac[WF_LESS]
+   >> `WF (λ(x:num list) y.
+            list_size (\n. n) x < list_size (\n. n) y)` by (
+       qabbrev_tac `f = \x:num list. list_size (\n. n) x`
+       >> `inv_image ($<) f =
+            (λx:num list y.
+              list_size (λn. n) x < list_size (λn. n) y)` by (
+           simp[inv_image_def]
+       )
+       >> `WF (inv_image ($<) f)` suffices_by fs[]
+       >> metis_tac[WF_inv_image]
+   )
+   >> qabbrev_tac `P = (λs t. s ⊂ t ∧ s ⊆ tempSubForms g ∧ t ⊆ tempSubForms g)`
+   >> qabbrev_tac
+         `Q = (λ x y.
+                list_size (λn. n) x < list_size (λn. n) y)`
+   >> qabbrev_tac `f = λ a. tempSubForms g DIFF {x | inAuto a x }`
+   >> `inv_image P f = λ a a2.
+                        (tempSubForms g DIFF {x | inAuto a x }
+                         ⊂ tempSubForms g DIFF {x | inAuto a2 x })` by (
+      qunabbrev_tac `P`
+      >> fs[inv_image_def]
+      >> `(\x y. f x ⊂ f y) = (λa a2. f a ⊂ f a2)`
+         suffices_by (
+          fs[] >> qunabbrev_tac `f` >> simp[inv_image_def]
+      )
+      >> metis_tac[]
+   )
+   >> `WF (inv_image P f)` by metis_tac[WF_inv_image]
+   >> `WF (P LEX Q)` by metis_tac[WF_LEX]
+   >> qabbrev_tac
+        `j = λ(a,l:num list). (tempSubForms g DIFF {x | inAuto a x},l)`
+   >> `WF (inv_image (P LEX Q) j)` by metis_tac[WF_inv_image]
+   >> `!x y. (NoNodeProcessedTwice g) x y ==> (inv_image (P LEX Q) j) x y` by (
+       fs[inv_image_def,LEX_DEF] >> rpt strip_tac
+         >> Cases_on `x` >> Cases_on `y` >> fs[NoNodeProcessedTwice_def]
+         >> qunabbrev_tac `f` >> qunabbrev_tac `P` >> qunabbrev_tac `Q`
+         >> simp[] >> simp[EQ_IMP_THM] >> rpt strip_tac
+         >> (qunabbrev_tac `j` >> simp[])
+   )
+   >> metis_tac[WF_SUBSET]
+ );
 
 
 
